src/Language/PlutusIR/Semantics/Static/Weakening.v
@@ -1,0 +1,304 @@
+Require Import PlutusCert.Language.PlutusIR.
+Import NamedTerm.
+Require Import PlutusCert.Language.PlutusIR.Semantics.Static.
+Require Import PlutusCert.Language.PlutusIR.Semantics.Static.Implementations.Named.
+
+Import Coq.Strings.String.
+Local Open Scope string_scope.
+
+Definition inclusion (ctx1 ctx2 : Context) : Prop :=
+  (forall x T, lookupT ctx1 x = Coq.Init.Datatypes.Some T -> lookupT ctx2 x = Coq.Init.Datatypes.Some T) /\
+  (forall X K, lookupK ctx1 X = Coq.Init.Datatypes.Some K -> lookupK ctx2 X = Coq.Init.Datatypes.Some K).
+
+Lemma inclusion_empty : forall ctx2,
+    inclusion empty ctx2.
+Proof.
+  intros.
+  unfold inclusion.
+  simpl.
+  split; intros; inversion H.
+Qed.
+
+Lemma inclusion_extendT : forall (ctx1 ctx2 : Context) (y : binderName) (T : Ty),
+    inclusion ctx1 ctx2 ->
+    inclusion (extendT y T ctx1) (extendT y T ctx2).
+Proof.
+  unfold inclusion.
+  intros.
+  split.
+  - intros.
+    unfold lookupT.
+    simpl.
+    unfold lookupT in H0.
+    simpl in H0.
+    destruct (x =? y) eqn:Hxy.
+    + assumption.
+    + fold lookupK.
+      fold lookupK in H0.
+      apply H.
+      assumption.
+  - intros. 
+    simpl.
+    apply H.
+    assumption.
+Qed.
+
+Lemma inclusion_extendK : forall (ctx1 ctx2 : Context) (y : binderTyname) (K : Kind),
+    inclusion ctx1 ctx2 ->
+    inclusion (extendK y K ctx1) (extendK y K ctx2).
+Proof.
+  unfold inclusion.
+  intros.
+  split.
+  - intros.
+    simpl.
+    apply H.
+    assumption.
+  - intros.
+    unfold lookupK.
+    simpl.
+    unfold lookupK in H0.
+    simpl in H0.
+    destruct (X =? y) eqn:Hxy.
+    + assumption.
+    + fold lookupK.
+      fold lookupK in H0.
+      apply H.
+      assumption.
+Qed.
+
+Lemma inclusion_append : forall (ctx1 ctx2 ctx' : Context),
+    inclusion ctx1 ctx2 ->
+    inclusion (Named.append ctx' ctx1) (Named.append ctx' ctx2).
+Proof.
+  intros.
+  induction ctx'.
+  - simpl.
+    assumption.
+  - unfold Named.append.
+    simpl.
+    split.
+    + destruct a; destruct p.
+      * intros x T. 
+        unfold lookupT.
+        fold lookupT.
+        destruct (x =? s) eqn:Hxy.
+        -- auto.
+        -- intros.
+           apply IHctx'.
+           assumption.
+      * intros x T.
+        apply IHctx'.
+    + destruct a; destruct p.
+      * intros xT.
+        apply IHctx'.
+      * intros x T.
+        unfold lookupK.
+        fold lookupK.
+        destruct (x =? s) eqn:Hxy.
+        -- auto.
+        -- intros.
+           apply IHctx'.
+           assumption.
+Qed.
+      
+Lemma weakening__has_kind : forall ctx ctx' T K,
+    inclusion ctx ctx' ->
+    ctx |-* T : K ->
+    ctx' |-* T : K.
+Proof.
+  intros ctx ctx' T K H HT.
+  generalize dependent ctx'.
+  induction HT; intros; eauto using inclusion_extendK with typing.
+  - apply K_Var.
+    apply H0.
+    apply H.
+Qed.
+
+
+Definition P_has_type ctx t T : Prop :=
+  forall ctx',
+    inclusion ctx ctx' ->
+    ctx' |-+ t : T.
+
+Definition P_constructor_well_formed ctx c : Prop :=
+  forall ctx',
+    inclusion ctx ctx' ->
+    ctx' |-ok_c c.
+
+Definition P_bindings_well_formed_nonrec ctx bs : Prop :=
+  forall ctx',
+    inclusion ctx ctx' ->
+    ctx' |-oks_nr bs.
+
+Definition P_bindings_well_formed_rec ctx bs : Prop :=
+  forall ctx',
+    inclusion ctx ctx' ->
+    ctx' |-oks_r bs.
+
+Definition P_binding_well_formed ctx b : Prop :=
+  forall ctx',
+    inclusion ctx ctx' ->
+    ctx' |-ok b.
+
+Lemma weakening : 
+  (forall ctx t T, ctx |-+ t : T -> P_has_type ctx t T) /\
+  (forall ctx bs, ctx |-oks_nr bs -> P_bindings_well_formed_nonrec ctx bs) /\
+  (forall ctx bs, ctx |-oks_r bs -> P_bindings_well_formed_rec ctx bs) /\
+  (forall ctx b, ctx |-ok b -> P_binding_well_formed ctx b).
+Proof.
+  apply has_type__multind with 
+    (P := P_has_type) 
+    (P0 := P_constructor_well_formed)
+    (P1 := P_bindings_well_formed_nonrec)
+    (P2 := P_bindings_well_formed_rec)
+    (P3 := P_binding_well_formed).
+  - (* T_Let *)
+    intros. unfold P_has_type. intros.
+    eapply T_Let.
+    + reflexivity.
+    + apply H1.
+      assumption.
+    + apply H3.
+      subst.
+      apply inclusion_append.
+      assumption.
+  - (* T_LetRec *)
+    intros. unfold P_has_type. intros.
+    eapply T_LetRec.
+    + reflexivity.
+    + apply H1.
+      subst.
+      apply inclusion_append.
+      assumption.
+    + apply H3.
+      subst.
+      apply inclusion_append.
+      assumption.
+  - (* T_Var *)
+    intros. unfold P_has_type. intros.
+    apply T_Var.
+    apply H0.
+    assumption.
+  - (* T_TyAbs *)
+    intros. unfold P_has_type. intros.
+    apply T_TyAbs.
+    apply H0.
+    apply inclusion_extendK.
+    assumption.
+  - (* T_LamAbs *)
+    intros. unfold P_has_type. intros.
+    apply T_LamAbs.
+    + apply H0.
+      apply inclusion_extendT.
+      assumption.
+    + apply weakening__has_kind with ctx.
+      * assumption.
+      * assumption.
+  - (* T_Apply *)
+    intros. unfold P_has_type. intros.
+    apply T_Apply with T1.
+    + apply H0.
+      assumption.
+    + apply H2.
+      assumption.
+  - (* T_Constant *)
+    intros. unfold P_has_type. intros.
+    apply T_Constant.
+  - (* T_Builtin *)
+    intros. unfold P_has_type. intros.
+    apply T_Builtin.
+  - (* T_TyInst *)
+    intros. unfold P_has_type. intros.
+    apply T_TyInst with (T1 := T1) (X := X) (K2 := K2).
+    + apply H0.
+      assumption.
+    + apply weakening__has_kind with ctx.
+      * assumption.
+      * assumption.
+    + assumption.
+  - (* T_Error *)
+    intros. unfold P_has_type. intros.
+    apply T_Error.
+    apply weakening__has_kind with ctx.
+    + assumption.
+    + assumption.
+  - (* T_IWrap *)
+    intros. unfold P_has_type. intros.
+    apply T_IWrap with X K S.
+    + assumption.
+    + apply H1.
+      assumption.
+    + apply weakening__has_kind with ctx.
+      * assumption.
+      * assumption.
+    + apply weakening__has_kind with ctx. 
+      * assumption.
+      * assumption.
+  - (* T_Unwrap *)
+    intros. unfold P_has_type. intros.
+    apply T_Unwrap with F X K T.
+    + apply H0.
+      assumption.
+    + apply weakening__has_kind with ctx.
+      * assumption.
+      * assumption.
+    + assumption.
+
+  - (* W_Con *)
+    intros. unfold P_constructor_well_formed. intros.
+    apply W_Con.
+    intros.
+    apply weakening__has_kind with ctx.
+    + assumption.
+    + apply H.
+      assumption.
+  
+  - (* W_NilB_NonRec *)
+    intros. unfold P_bindings_well_formed_nonrec. intros.
+    apply W_NilB_NonRec.
+  - (* W_ConsB_NonRec *)
+    intros. unfold P_bindings_well_formed_nonrec. intros.
+    apply W_ConsB_NonRec.
+    + apply H0.
+      assumption.
+    + apply H2.
+      apply inclusion_append.
+      assumption.
+  
+  - (* W_NilB_Rec *)  
+    intros. unfold P_bindings_well_formed_rec. intros.
+    apply W_NilB_Rec.
+  - (* W_ConsB_Rec *)
+    intros. unfold P_bindings_well_formed_rec. intros.
+    apply W_ConsB_Rec.
+    + apply H0.
+      assumption.
+    + apply H2.
+      assumption.
+  
+  - (* W_Term *)
+    intros. unfold P_binding_well_formed. intros.
+    apply W_Term.
+    + apply weakening__has_kind with ctx.
+      * assumption.
+      * assumption.
+    + apply H1.
+      assumption.
+  - (* W_Type *)
+    intros. unfold P_binding_well_formed. intros.
+    apply W_Type.
+    apply weakening__has_kind with ctx.
+    + assumption.
+    + assumption.
+  - (* W_Data *)
+    intros. unfold P_binding_well_formed. intros.
+    eapply W_Data.
+    + reflexivity.
+    + intros.
+      apply H1.
+      * assumption.
+      * subst.
+        apply inclusion_append.
+        assumption.
+Qed.
